DbAppProgramLogic/Refinement.lean
@@ -1,4 +1,4 @@
-import DbAppProgramLogic.Transformer
+import DbAppProgramLogic.Legacy
 import DbAppProgramLogic.Server
 
 namespace DbAppProgramLogic
